coqimp/contextswitch/lib/derived_rule.v
@@ -27,8 +27,6 @@ Require Import reg_lemma.
 Open Scope nat.
 Open Scope code_scope.
 Open Scope mem_scope.
-  
-Print wf_seq.
 
 Theorem forward_rule :
   forall p q q' Spec I,
@@ -64,11 +62,50 @@ Proof.
   eauto.
 Qed.
 
+Theorem disj_sep_rule :
+  forall p1 p2 p q I Spec,
+    Spec |- {{ p1 ** p }} I {{ q }} ->
+           Spec |- {{ p2 ** p }} I {{ q }} ->
+                  Spec |- {{ (p1 \\// p2) ** p }} I {{ q }}.
+Proof.
+  intros.
+  assert (Ht : Spec |- {{(p1 ** p) \\// (p2 ** p)}} I {{q \\// q}}).
+  {
+    eapply Seq_disj_rule; eauto.
+  }
+  eapply Seq_conseq_rule.
+  eapply Ht.
+  clear.
+  introv Hs.
+  sep_star_split_tac.
+  simpl in H3.
+  simpljoin1.
+  simpl in H1.
+  simpl.
+  destruct H1.
+  left.
+  do 2 eexists.
+  simpl; repeat (split; eauto).
+  right.
+  do 2 eexists.
+  simpl; repeat (split; eauto).
+  introv Hs.
+  simpl in Hs; destruct Hs; eauto.
+Qed.
+
 Ltac hoare_ex_intro :=
   match goal with
   | |- _ |- {{ EX _, _ }} _ {{ EX _, _ }} =>
     eapply ex_intro_rule'; try intros;
     hoare_ex_intro
+  | _ => idtac
+  end.
+
+Ltac hoare_ex_intro_pre :=
+  match goal with
+  | |- _ |- {{ EX _, _ }} _ {{ _ }} =>
+    eapply Ex_intro_rule; try intros;
+    hoare_ex_intro_pre
   | _ => idtac
   end.
 
@@ -78,5 +115,269 @@ Ltac hoare_lift_pre n :=
   | |- _ |- {{ _ }} _ {{ _ }} =>
     eapply backward_rule;
     [ introv H'; simpl_sep_liftn_in H' n; eapply H' | idtac]
+  | _ => idtac
+  end.
+
+Theorem aexists_intro :
+  forall {t : Type} (P : t->asrt) s,
+  (exists x, s |= P x) -> s |= EX x, P x.
+Proof.
+  intros.
+  simpljoin1.
+  simpl; eauto.
+Qed.
+
+Theorem aexists_elim :
+  forall {t : Type} (P : t->asrt) s,
+    s |= EX x, P x -> (exists x, s |= P x).
+Proof.
+  intros.
+  simpls; eauto.
+Qed.
+
+Theorem astar_r_aexists_intro :
+  forall {t:Type} P (Q:t->asrt),
+    EX x, (P ** Q x) ==> P ** EX x, Q x.
+Proof.
+  intros.
+  simpls.
+  simpljoin1.
+  destruct_state x0.
+  destruct_state x1.
+  simpls.
+  simpljoin1.
+  exists (m, (r, f0), d0) (m0, (r0, f0), d0).
+  simpl; repeat (split; eauto).
+Qed.
+
+Theorem astar_l_aexists_intro :
+  forall {t:Type} (P:t->asrt) Q,
+    EX x, (P x ** Q) ==> (EX x, P x) ** Q.
+Proof.
+  intros.
+  simpls.
+  simpljoin1.
+  destruct_state x0.
+  destruct_state x1.
+  simpls.
+  simpljoin1.
+  exists (m, (r, f0), d0) (m0, (r0, f0), d0).
+  simpl; repeat (split; eauto).
+Qed.
+
+Theorem astar_r_aexists_elim :
+  forall {t:Type} P (Q:t->asrt),
+    P ** (EX x, Q x) ==> EX x, (P ** Q x).
+Proof.
+  intros.
+  simpl in *.
+  simpljoin1.
+  destruct_state x.
+  destruct_state x0.
+  simpls.
+  simpljoin1.
+  exists x1 (m, (r, f0), d0) (m0, (r0, f0), d0).
+  simpl; repeat (split; eauto).
+Qed.
+
+Theorem astar_l_aexists_elim :
+  forall {t:Type} (P:t->asrt) Q,
+    (EX x, P x) ** Q ==> EX x, (P x ** Q).
+Proof.
+  intros.
+  simpl in *.
+  simpljoin1.
+  destruct_state x.
+  destruct_state x0.
+  simpls.
+  simpljoin1.
+  exists x1 (m, (r, f0), d0) (m0, (r0, f0), d0).
+  simpl; repeat (split; eauto).
+Qed.
+
+Theorem aconj_r_aexists_intro :
+  forall {t:Type} P (Q:t->asrt),
+    EX x, (P //\\ Q x) ==> P //\\ EX x, Q x.
+Proof.
+  intros.
+  simpl in *.
+  simpljoin1.
+  split; eauto.
+Qed.
+
+Theorem aconj_l_aexists_intro :
+  forall {t:Type} (P:t->asrt) Q,
+    EX x, (P x //\\ Q) ==> (EX x, P x) //\\ Q.
+Proof.
+  intros.
+  simpl in *.
+  simpljoin1.
+  split; eauto.
+Qed.
+
+Theorem aconj_r_aexists_elim :
+  forall {t:Type} P (Q:t->asrt),
+    P //\\ (EX x, Q x) ==> EX x, (P //\\ Q x).
+Proof.
+  intros.
+  simpl in *.
+  simpljoin1; eauto.
+Qed.
+
+Theorem aconj_l_aexists_elim :
+  forall {t:Type} (P:t->asrt) Q,
+    (EX x, P x) //\\ Q ==> EX x, (P x //\\ Q).
+Proof.
+  intros.
+  simpl in *.
+  simpljoin1; eauto.
+Qed.
+
+Theorem adisj_r_aexists_intro :
+  forall {t:Type} P (Q:t->asrt),
+    EX x, (P \\// Q x) ==> P \\// EX x, Q x.
+Proof.
+  intros.
+  simpl in *.
+  simpljoin1.
+  destruct H; eauto.
+Qed.
+
+Theorem adisj_l_aexists_intro :
+  forall {t:Type} (P:t->asrt) Q,
+    EX x, (P x \\// Q) ==> (EX x, P x) \\// Q.
+Proof.
+  intros.
+  simpl in *.
+  simpljoin1.
+  destruct H; eauto.
+Qed.
+
+Theorem adisj_r_aexists_elim :
+  forall {t:Type} P (Q:t->asrt),
+    (exists (x:t), x = x) ->
+    P \\// (EX x, Q x) ==> EX x, (P \\// Q x).
+Proof.
+  intros.
+  simpls. 
+  simpljoin1.
+  destruct H0; eauto.
+  simpljoin1.
+  eauto.
+  Unshelve.
+  exact x.
+Qed.
+
+Theorem adisj_l_aexists_elim :
+  forall {t:Type} (P:t->asrt) Q,
+    (exists (x:t), x = x) ->
+    (EX x, P x) \\// Q ==> EX x, (P x \\// Q).
+Proof.
+  intros.
+  simpls.
+  simpljoin1.
+  destruct H0; eauto.
+  simpljoin1; eauto.
+  Unshelve.
+  exact x.
+Qed.
+
+Ltac sep_ex_intro :=
+  match goal with
+  | |- ?s |= (EX _, _) =>
+    eapply aexists_intro; eexists; sep_ex_intro
+  | |- ?s |= (EX _, _) ** ?p =>
+    eapply astar_l_aexists_intro; sep_ex_intro
+  | |- ?s |= ?p ** (EX _, _) =>
+    eapply astar_r_aexists_intro; sep_ex_intro
+  | |- ?s |= (EX _, _) //\\ ?p =>
+    eapply aconj_l_aexists_intro; sep_ex_intro
+  | |- ?s |= ?p //\\ (EX _, _) =>
+    eapply aconj_r_aexists_intro; sep_ex_intro
+  | |- ?s |= (EX _, _) \\// ?p =>
+    eapply adisj_l_aexists_intro; sep_ex_intro
+  | |- ?s |= ?p \\// (EX _, _) =>
+    eapply adisj_r_aexists_intro; sep_ex_intro
+  | _ => idtac
+  end.
+
+Theorem sep_pure_l_intro :
+  forall (pu : Prop) p s,
+    pu -> s |= p -> s |= [| pu |] ** p.
+Proof.
+  intros.
+  simpl.
+  destruct_state s.
+  exists (empM, (empR, f), d) (m, (r, f), d).
+  simpl; repeat (split; eauto).
+  unfold disjoint.
+  intros; eauto.
+  simpl.
+  destruct (m x); eauto.
+  unfold disjoint.
+  intros; eauto.
+  simpl.
+  destruct (r x); eauto.
+Qed.
+
+Theorem sep_pure_r_intro :
+  forall (pu : Prop) p s,
+    pu -> s |= p -> s |= p ** [| pu |].
+Proof.
+  intros.
+  destruct_state s.
+  simpl.
+  exists (m, (r, f), d) (empM, (empR, f), d).
+  simpl; repeat (split; eauto).
+  unfold disjoint.
+  intros.
+  destruct (m x); simpl; eauto.
+  unfold disjoint.
+  intros.
+  destruct (r x); simpl; eauto.
+  rewrite merge_empR_r_eq; eauto.
+  rewrite merge_empM_r_eq; eauto.
+Qed.
+
+Theorem sep_pure_l_elim :
+  forall (pu : Prop) p s,
+    s |= [| pu |] ** p -> pu /\ s |= p.
+Proof.
+  intros.
+  sep_star_split_tac.
+  simpls.
+  simpljoin1.
+  split; eauto.
+Qed.
+
+Theorem sep_pure_r_elim :
+  forall (pu : Prop) p s,
+    s |= p ** [| pu |] -> pu /\ s |= p.
+Proof.
+  intros.
+  sep_star_split_tac.
+  simpls.
+  simpljoin1.
+  split; eauto.
+  rewrite empM_merge_still_r; eauto.
+  rewrite merge_empR_r_eq; eauto.
+Qed.
+
+Ltac sep_ex_elim_in H :=
+  match type of H with
+  | ?s |= (EX _, _) =>
+    eapply aexists_elim in H; destruct H as [?x H]; sep_ex_elim_in H
+  | ?s |= (EX _, _) ** ?p =>
+    eapply astar_l_aexists_elim in H; destruct H as [?x H]; sep_ex_elim_in H
+  | ?s |= ?p ** (EX _, _) =>
+    eapply astar_r_aexists_elim in H; destruct H as [?x H]; sep_ex_elim_in H
+  | ?s |= (EX _, _) //\\ ?p =>
+    eapply aconj_l_aexists_elim in H; destruct H as [?x H]; sep_ex_elim_in H
+  | ?s |= ?p //\\ (EX _, _) =>
+    eapply aconj_r_aexists_elim in H; destruct H as [?x H]; sep_ex_elim_in H
+  | ?s |= (EX _, _) \\// ?p =>
+    eapply adisj_l_aexists_elim in H; destruct H as [?x H]; sep_ex_elim_in H
+  | ?s |= ?p \\// (EX _, _) =>
+    eapply adisj_r_aexists_elim in H; destruct H as [?x H]; sep_ex_elim_in H
   | _ => idtac
   end.
