coqimp/contextswitch/proof/CtxSwitchProof.v
@@ -1,0 +1,444 @@
+Require Import Coqlib.                 
+Require Import Maps.         
+Require Import LibTactics.   
+        
+Require Import Integers.  
+Open Scope Z_scope.      
+Import ListNotations.  
+  
+Set Asymmetric Patterns.  
+        
+Require Import state.    
+Require Import language. 
+ 
+Set Implicit Arguments.    
+Unset Strict Implicit. 
+              
+Require Import logic.
+    
+Require Import lemmas.
+Require Import lemmas_ins.
+
+Require Import Coq.Logic.FunctionalExtensionality.
+
+Require Import sep_lemma.
+Require Import reg_lemma.
+Require Import derived_rule.
+
+Require Import code.
+Require Import ctxswitch_spec.
+
+Open Scope nat.
+Open Scope code_scope.
+Open Scope mem_scope.
+
+Definition spec := convert_spec
+                     ((Ta0_return, Ta0_return +ᵢ ($ 4),
+                       (os_ta0_return_pre, os_ta0_return_post)) :: nil).
+
+(*+ Lemmas about TimReduce +*)
+Theorem GenRegs_TimeReduce :
+  forall grst p,
+    (GenRegs grst ** p) ↓ = GenRegs grst ** (p ↓).
+Proof.
+  intros.
+  simpl.
+  destruct grst.
+  destruct p0.
+  destruct p0.
+  destruct f1, f2, f0, f.
+  simpl.
+  eauto.
+Qed.
+
+Theorem FrameState_TimeReduce :
+  forall id vi F p,
+    (FrameState id vi F ** p) ↓ = FrameState id vi F ** (p ↓).
+Proof.
+  intros.
+  simpls.
+  unfold FrameState.
+  eauto.
+Qed.
+
+Theorem RegSt_TimeReduce :
+  forall rn v p,
+    (rn |=> v ** p) ↓ = rn |=> v ** (p ↓).
+Proof.
+  intros.
+  simpl; eauto.
+Qed.
+
+Theorem MemSto_TimeReduce :
+  forall l v p,
+    (l |-> v ** p) ↓ = l |-> v ** (p ↓).
+Proof.
+  intros.
+  simpl; eauto.
+Qed.
+
+Lemma save_reg_TimeReduce' :
+  forall n l vl,
+    save_reg l n vl ↓ = save_reg l n vl.
+Proof.
+  intro n.
+  induction n; intros.
+  -
+    simpls.
+    destruct vl; eauto.
+  -
+    destruct vl.
+    {
+      simpl.
+      eauto.
+    }
+    {
+      simpl.
+      rewrite IHn; eauto.
+    }
+Qed.
+
+Lemma save_reg_TimeReduce :
+  forall n l vl p,
+    (save_reg l n vl ** p) ↓ = save_reg l n vl ** (p ↓).
+Proof.
+  intros.
+  simpl.
+  rewrite save_reg_TimeReduce'; eauto.
+Qed.
+
+Theorem Context_TimeReduce :
+  forall ctx p,
+    (context ctx ** p) ↓ = context ctx ** (p ↓).
+Proof.
+  intros.
+  simpls.
+  unfold context.
+  destruct ctx.
+  destruct p0.
+  destruct p0.
+  destruct p0.
+  unfold context'.
+  do 3 rewrite save_reg_TimeReduce.
+  simpl; eauto.
+Qed.
+
+Lemma stack_seg_TimeReduce :
+  forall l fm,
+    stack_seg l fm ↓ = stack_seg l fm.
+Proof.
+  intros.
+  destruct fm.
+  unfold stack_seg.
+  simpl; eauto.
+Qed.
+
+Lemma Stk_TimeReduce' :
+  forall lfp l,
+    stack' l lfp ↓ = stack' l lfp.
+Proof.
+  intro lfp.
+  induction lfp; intros.
+  -
+    simpl; eauto.
+  -
+    simpl.
+    destruct a.
+    simpl.
+    do 2 rewrite stack_seg_TimeReduce; eauto.
+    rewrite IHlfp; eauto.
+Qed.
+
+Theorem Stk_TimeReduce :
+  forall stk p,
+    (stack stk ** p) ↓ = stack stk ** (p ↓).
+Proof.
+  intros.
+  destruct stk.
+  unfold stack.
+  simpl.
+  rewrite Stk_TimeReduce'; eauto.
+Qed.
+
+Theorem conj_TimeReduce :
+  forall p1 p2,
+    (p1 //\\ p2) ↓ = (p1 ↓) //\\ (p2 ↓).
+Proof.
+  intros; eauto.
+Qed.
+
+Theorem disj_TimeReduce :
+  forall p1 p2,
+    (p1 \\// p2) ↓ = (p1 ↓) \\// (p2 ↓).
+Proof.
+  intros; eauto.
+Qed.
+
+Theorem pure_TimeReduce :
+  forall pu p,
+    ([| pu |] ** p) ↓ = [| pu |] ** (p ↓).
+Proof.
+  intros; eauto.
+Qed.
+
+Theorem Atrue_TimeReduce :
+  forall p,
+    (Atrue ** p) ↓ = Atrue ** (p ↓).
+Proof.
+  intros; eauto.
+Qed.
+
+Theorem Afalse_TimReduce :
+  forall p,
+    (Afalse ** p) ↓ = Afalse ** (p ↓).
+Proof.
+  intros; eauto.
+Qed.
+
+Ltac TimReduce_simpl :=
+  match goal with
+  | |- context [(GenRegs ?grst ** ?p) ↓] =>
+    rewrite GenRegs_TimeReduce; TimReduce_simpl
+  | |- context [(FrameState ?id ?vi ?F ** ?p) ↓] =>
+    rewrite FrameState_TimeReduce; TimReduce_simpl
+  | |- context [(?rn |=> ?v ** ?p) ↓] =>
+    rewrite RegSt_TimeReduce; TimReduce_simpl
+  | |- context [(?l |-> ?v ** ?p) ↓] =>
+    rewrite MemSto_TimeReduce; TimReduce_simpl
+  | |- context [(context ?ctx ** ?p) ↓] =>
+    rewrite Context_TimeReduce; TimReduce_simpl
+  | |- context [(stack ?stk ** ?p) ↓] =>
+    rewrite Stk_TimeReduce; TimReduce_simpl
+  | |- context [([| ?pu |] ** ?p) ↓] =>
+    rewrite pure_TimeReduce; TimReduce_simpl
+  | |- context [(Atrue ** ?p) ↓] =>
+    rewrite Atrue_TimeReduce; TimReduce_simpl
+  | |- context [(Afalse ** ?p) ↓] =>
+    rewrite Afalse_TimReduce; TimReduce_simpl
+  | |- context [(?p1 //\\ ?p2) ↓] =>
+    rewrite conj_TimeReduce; TimReduce_simpl
+  | |- context [(?p1 \\// ?p2) ↓] =>
+    rewrite disj_TimeReduce; TimReduce_simpl
+  | _ => simpl TimReduce
+  end.
+
+Ltac TimReduce_simpl_in H :=
+  match type of H with
+  | _ |= ?p =>
+    match p with
+    | context [(GenRegs ?grst ** ?p) ↓] =>
+      rewrite GenRegs_TimeReduce in H; TimReduce_simpl_in H
+    | context [(FrameState ?id ?vi ?F ** ?p) ↓] =>
+      rewrite FrameState_TimeReduce in H; TimReduce_simpl_in H
+    | context [(?rn |=> ?v ** ?p) ↓] =>
+      rewrite RegSt_TimeReduce in H; TimReduce_simpl_in H
+    | context [(?l |-> ?v ** ?p) ↓] =>
+      rewrite MemSto_TimeReduce in H; TimReduce_simpl_in H
+    | context [(context ?ctx ** ?p) ↓] =>
+      rewrite Context_TimeReduce in H; TimReduce_simpl_in H
+    | context [(stack ?stk ** ?p) ↓] =>
+      rewrite Stk_TimeReduce in H; TimReduce_simpl_in H
+    | context [([| ?pu |] ** ?p) ↓] =>
+      rewrite pure_TimeReduce in H; TimReduce_simpl_in H
+    | context [(Atrue ** ?p) ↓] =>
+      rewrite Atrue_TimeReduce in H; TimReduce_simpl_in H
+    | context [(Afalse ** ?p) ↓] =>
+      rewrite Afalse_TimReduce in H; TimReduce_simpl_in H
+    | context [(?p1 //\\ ?p2) ↓] =>
+      rewrite conj_TimeReduce in H; TimReduce_simpl_in H
+    | context [(?p1 \\// ?p2) ↓] =>
+      rewrite disj_TimeReduce in H; TimReduce_simpl_in H
+    | _ => simpl TimReduce in H
+    end
+  end.
+
+(*+ Lemmas about Integers +*)
+Lemma in_range4 :
+  ($ (-4096)) <=ᵢ ($ 4) && ($ 4) <=ᵢ ($ 4095) = true.
+Proof.
+  unfold orb.
+  unfold Int.lt.
+  unfold Int.eq.
+  destruct (zlt (Int.signed $ (-4096)) (Int.signed $ 4)) eqn:Heqe;
+    destruct (zeq (Int.unsigned $ (-4096)) (Int.unsigned $ 4)) eqn:Heqe1;
+    destruct (zlt (Int.signed $ 4) (Int.signed $ 4095)) eqn:Heqe2;
+    destruct (zeq (Int.unsigned $ 4) (Int.unsigned $ 4095)) eqn:Heqe3; eauto; tryfalse.
+Qed.
+
+Ltac eval_spec :=
+  match goal with
+  | |- ?spec (?f1, ?f2) = Some (?fp, ?fq) =>
+    unfold spec; unfold convert_spec;
+    repeat progress (destruct_addreq; destruct_addreq)
+  end.
+  
+(*+ Proof +*)
+Theorem OSInt0HandlerProof :
+  forall vl,
+    spec |- {{ os_int_ta0_handler_pre vl }}
+             os_int_ta0_handler
+           {{ os_int_ta0_handler_post vl }}.
+Proof.
+  intros.
+  unfold os_int_ta0_handler_pre.
+  unfold os_int_ta0_handler_post.
+  hoare_ex_intro_pre.
+  renames x' to fmg, x'0 to fmo, x'1 to fml, x'2 to fmi, x'3 to id, x'4 to F.
+  renames x'5 to vy, x'6 to vi, x'7 to bv, x'8 to ll.
+  renames x'9 to ct, x'10 to cctx, x'11 to cstk, x'12 to nt, x'13 to nctx, x'14 to nstk.
+  renames x'15 to vz, x'16 to vn.
+  eapply Pure_intro_rule; intros.
+  hoare_lift_pre 13.
+  eapply Pure_intro_rule; intros.
+  unfold os_int_ta0_handler.
+ 
+  eapply backward_rule.
+  introv Hs.
+  simpl_sep_liftn_in Hs 2.
+  eapply Regs_Global_combine_GenRegs in Hs; eauto.
+
+  (** add l1 4 l1 *)
+  destruct fmg.
+  destruct fmo.
+  destruct fml.
+  destruct fmi.
+  eapply seq_rule.
+  TimReduce_simpl.
+  simpl TimReduce.
+  eapply add_rule_reg; eauto.
+  instantiate (1 := ($ 4)).
+  simpl.
+  rewrite in_range4; eauto.
+
+  (** add l2 4 l2 *)
+  unfold l1 at 1 2.
+  simpl upd_genreg.
+  eapply seq_rule.
+  TimReduce_simpl.
+  eapply add_rule_reg; eauto.
+  simpl.
+  rewrite in_range4; eauto.
+
+  (** set OSTaskSwitch l4 *)
+  unfold l2 at 1 2.
+  simpl upd_genreg.
+  eapply seq_rule.
+  TimReduce_simpl.
+  eapply set_rule_reg; eauto.
+
+  (** ld [l4] l4 *)
+  simpl upd_genreg.
+  hoare_lift_pre 8.
+  hoare_lift_pre 2.
+  eapply seq_rule.
+  TimReduce_simpl.
+  eapply ld_rule_reg; eauto.
+  simpl upd_genreg.
+
+  (** set OSTRUE l5 *)
+  eapply seq_rule.
+  TimReduce_simpl.
+  eapply set_rule_reg; eauto.
+  simpl upd_genreg.
+
+  (** subcc l4 l5 g0 *)
+  hoare_lift_pre 5.
+  hoare_lift_pre 6.
+  hoare_lift_pre 3.
+  eapply seq_rule.
+  TimReduce_simpl.
+  eapply subcc_rule_reg; eauto.
+  simpl. eauto.
+  simpl upd_genreg.
+  simpl get_genreg_val at 1 2.
+
+  eapply backward_rule.
+  introv Hs.
+  simpl_sep_liftn_in Hs 12.
+  eauto.
+
+  match goal with
+  | H : get_frame_nth _ _ = Some _ |- _ =>
+    simpl in H; inversion H; subst
+  end.
+  eapply disj_sep_rule.
+  {
+    eapply backward_rule.
+    introv Hs.
+    eapply astar_assoc_elim in Hs; eauto.
+    eapply Pure_intro_rule; introv Hbv.
+    subst.
+    assert (Hnzero : iszero OSFALSE -ᵢ OSTRUE = $ 0).
+    {
+      unfold Int.sub, OSFALSE, OSTRUE.
+      unfold iszero.
+      destruct (Int.eq_dec $ (Int.unsigned $ 0 - Int.unsigned $ 1) $ 0) eqn:Heqe; eauto.
+      clear Heqe.
+      inversion e; eauto.
+    }
+    rewrite Hnzero.
+
+    (** bne Ta0_return; nop *)
+    eapply Bne_rule; eauto.
+    {
+        eval_spec.
+    }
+    {
+      eapply nop_rule; eauto.
+    }
+    {
+      introv Hs.
+      TimReduce_simpl_in Hs.
+      sep_cancel1 4 1.
+      simpl; eauto.
+    }
+    { 
+      introv Hcontr.
+      rewrite Int.eq_true in Hcontr; tryfalse.
+    }
+
+    Focus 2.
+    introv Htrue.
+    split.
+    {
+      introv Hs.
+      TimReduce_simpl_in Hs.
+      unfold os_ta0_return_pre. 
+      sep_ex_intro.
+      eapply astar_assoc_intro.
+      eapply sep_pure_l_intro.
+      Focus 2.
+      eapply astar_assoc_intro.
+      sep_cancel1 2 1.
+      simpl_sep_liftn_in H 5.
+      eauto.
+      eauto.
+    }
+    {
+      introv Hs.
+      unfold os_ta0_return_post in Hs.
+      sep_ex_intro.
+      sep_ex_elim_in Hs.
+      eapply astar_assoc_elim in Hs.
+      eapply sep_pure_l_elim in Hs.
+      destruct Hs as [Hlg Hs].
+      inversion Hlg; subst.
+      simpl upd_genreg in Hs.
+      eapply sep_pure_l_intro.
+      eauto.
+      eapply astar_assoc_elim in Hs.
+      sep_cancel1 2 3.
+      sep_cancel1 6 3.
+      sep_cancel1 4 3.
+      sep_cancel1 3 3.
+      sep_cancel1 4 3.
+      sep_cancel1 3 4.
+      sep_cancel1 3 3.
+      sep_cancel1 3 3.
+      sep_cancel1 3 3.
+      sep_cancel1 3 3.
+      
+    }
+  }
+    
+  >>>>>>>>>>>>>>>
